#+TITLE: Homework 1
#+AUTHOR: Alexander Brown
#+DATE: \today

#+OPTIONS: toc:nil
#+BIND: org-export-latex-title-command ""
#+LATEX: \setcounter{secnumdepth}{-1}

# =========================================================================================================================
# Babel properties

#+PROPERTY: header-args:octave :session *octave* :results output :exports both

# =========================================================================================================================
# Org LaTeX options

#+OPTIONS: tex:t
#+LATEX_CLASS: article

#+latex_header: \pagestyle{fancy}
#+latex_header: \fancyhead{}
#+latex_header: \rhead{\textit{Alexander Brown}}
#+latex_header: \lhead{\textit{ECE 6030}}
#+latex_header: \small
#+latex_header: \usepackage{amsfonts}                       % Cool math fonts
#+latex_header: \usepackage{amsmath}                        % Maths
#+latex_header: \setlength\parindent{0pt}                   % No indent for paragraphs

#+latex_header: \newcommand{\shall}{\textbf{shall }}

# =========================================================================================================================
# More document configuration

#+begin_export latex
\parskip 3mm                                % Set the vetical space between paragraphs
\let\ref\autoref                            % Redifine `\ref` as `\autoref` because lazy
#+end_export

* 3
** Problem Statement
Show that the following are convex:

1. The set of $n \times n$ Toeplitz matrices
2. The set of monic polynomials of the same degree
3. The set of symmetric matrices

** Solution
Begin by defining what a complex set is:

#+begin_quote
A set $S$ is convex if for any two points $p,q \in S$, then all points of the form

$$
\lambda p + (1 - \lambda)q
$$

for $0 \le \lambda \le 1$, are also in $S$.
#+end_quote

*** 3.1: Toeplitz
:PROPERTIES:
:CUSTOM_ID: sec:3.1
:END:

Begin by defining what a Toeplitz matrix is

#+begin_quote
A Toeplitz matrix is a diagonal-constant matrix, which means all elements along a diagonal have the same value. For a
Toeplitz matrix $A$ we have $A_{ij} = a_{i-j}$ which results in the form

\begin{equation*}
\begin{bmatrix}
a & b & c & \cdots \\
e & a & b & \cdots \\
f & e & a & \cdots \\
\vdots & \vdots & \vdots & \ddots
\end{bmatrix}
\end{equation*}
#+end_quote

Consider Toeplitz matrices $P$ and $Q$ of dimension $n \times n$ as let $S$ be the set of $n\times n$ Toeplitz matrices. Lets now apply the definition of the convex set:

$$
\lambda P + (1 - \lambda)Q
$$

There are two operations being applied to the matrices: addition

#+begin_quote
If $A = [a_{ij}]$ and $B = [b_{ij}]$ are matrices of the same size, then their sum $A+B$ is the matrix obtained by
adding the corresponding elements of the matrix $A$ and $B$.
#+end_quote

and multiplication of a matrix by a number

#+begin_quote
If $A = [a_ij]$ is a matrix and $c$ is a number, then $cA$ is the matrix obtained by multiplying each element of $A$ by
$c$.
#+end_quote

Therefore, we can make the statements

- Any Toeplitz matrix multiplied by a scalar is also Toeplitz
- Any two $n \times n$ Toeplitz matrices being added together is also Toeplitz

The following statement can then be made: The set of $n \times n$ Toeplitz matrices is convex.

$$
\lambda P + (1 - \lambda)Q \in S
$$

*** 3.2: Monic Polynomials of Degree $n$
Begin by defining what a monic polynomial is

#+begin_quote
A polynomial is monic if the coefficient of the highest order term is 1.
#+end_quote

Suppose $p$ and $q$ are monic polynomials of degree $n$ and $S$ is the set of all monic polynomials of degree $n$. It
can be written

$$
\lambda p(x) + (1 - \lambda)q(x) \in S
$$

Expanding the above gives

\begin{equation*}
\begin{array}{l}
\lambda (x^n - ax^{n-1} + \cdots + bx + c) + (1- \lambda)(x^n + dx^{n-1} + \cdots + ex + f) \\
= 2 \lambda x^n + (a+d x^{n-1}) + \cdots \\
\end{array}
\end{equation*}

Dividing by $2\lambda$ produces another monic polynomial of degree $n$. Therefore, the set is convex, i.e $\lambda p(x) + (1 - \lambda)q(x) \in S$.

*** 3.3: Symmetric Matrices
Define what a symmetric matrix is

#+begin_quote
A matrix $A$ is symmetric $\iff A = A^T$.
#+end_quote

Similarly to [[#sec:3.1][3.1]],

- Let $P$ and $Q$ are $n \times n$ symmetric matrices
- $S$ is the set of $n \times n$ symmetric matrices
- Any symmetric matrix multiplied by a scalar is also symmetric
- Any two $n \times n$ symmetric matrices being added together is also symmetric

Therefore, $S$ is convex because $\lambda P + (1 - \lambda)Q \in S$.

* 4
** Problem Statement
The set of even integers can be represented as $2\mathbb{Z}$. Show that $|2\mathbb{Z}| = |\mathbb{Z}|$. Similarly show that there are as many odd
integers as there are integers.

** Solution
Let $S$ and $T$ be two different sets. $T$ and $S$ have the same cardinality if there is a bijection $f$ from $S$ to
$T$. Therefore, we need to show $f : \mathbb{Z} \rightarrow 2\mathbb{Z}$. Let the mapping $f(n)$ be defined as

\begin{equation*}
f(n) = 2n
\end{equation*}

It now needs to be shown that $f(n)$ is both one-to-one and onto. To show that $f(n)$ is one-to-one begin by defining
how to show a mapping is one-to-one

#+begin_quote
A function $f$ from $A$ onto $B$ is one-to-one if each element of $B$ has at most one element of $A$ mapped into it.
That is, $f(x) = f(y)$, then $x = y$.
#+end_quote

From this if we suppose $f(a) = f(b)$, then $2a = 2b$ so $a=b$. Thus, $f$ is one-to-one. Now we need to show $f$ is
onto. Begin by defining onto

#+begin_quote
A function is onto if each element of $B$ has at least one element of $A$ that is mapped into it. That is, $\forall b
\in B$ there is an $a \in A$ such that $f(a) = b$.
#+end_quote

Take $b = 2n$ for some $a$, then $f(n) = 2n = b$ which shows that $f$ is onto. Therefore, $f(n)$ is a bijection and
$|\mathbb{Z}| = |2\mathbb{Z}|$.

Similarly, for the odd we need to show $f : \mathbb{Z} \rightarrow 2\mathbb{Z}+1$ is a bijection. To show $f(n)$ is one-to-one let $f(a) = f(b)$,
then $2a + 1 = 2b + 1$, so $a=b$. To show $f$ is onto let $b = 2n+1$, then $f(n) = 2n + 1 = b$. Therefore, $f(n)$ is a
bijection and $|\mathbb{Z}| = |2\mathbb{Z}+1|$.

* 5

** Problem Statement
Show that $|(0,1]| = |\mathbb{R}|$.

** Solution
A simple way to go about this is to first show that $\big|[0,1)\big| = \big|[-\pi/2, \pi/2)\big|$. Suppose $f(x) = \pi x - \pi/2$. To show that
$f(x)$ is one-to-one

\begin{equation*}
\begin{array}{l}
f(x) = f(y) \\
\pi x - \pi/2 = \pi y - \pi/2 \\
\pi x = \pi y \\
x = y
\end{array}
\end{equation*}

Therefore, $f(x)$ is one-to-one. Now to show that $f(x)$ is also onto.

\begin{equation*}
\begin{array}{l}
f(x) = y \\
\pi x - \pi / 2 = y \\
x = y/\pi + 1/2
\end{array}
\end{equation*}

And because we know that $0 < x \le 1$ we can show that $x$ written above is in that range by saying

\begin{equation*}
\begin{array}{l}
- \pi/2 < y \le \pi/2 \\
- 1/2 < y/\pi \le 1/2 \\
0 < y/\pi + 1/2 \le 1\\
\end{array}
\end{equation*}

Therefore, the function is also onto. Now to show that $\big|[-\pi/2, \pi/2)\big| = \big| \mathbb{R} \big|$. Let $g(x) = tan(x)$ it
can be shown that $tan(x)$ is always increasing.

#+begin_quote
*Fact*: If $g(x)$ is always increasing, then $g(x)$ is one-to-one.
#+end_quote

By taking the derivative of $g'(x) = sec^2(x) > 0$, therefore $g(x)$ is one-to-one. To show that $g(x)$ is onto, we will
use the intermediate value theorem

#+begin_quote
If $g(x)$ is continuous on an interval $[a,b]$, then $g(x)$ contains all the values between $g(a)$ and $g(b)$.
#+end_quote

Let the range of interest be $[-\pi/2 + \epsilon, \pi/2 - \epsilon]$. $g(x)$ is continuous within the range, therefore it obtains all
values $g(-\pi/2 + \epsilon)$ to $g(\pi/2 - \epsilon)$. If we let $\epsilon \rightarrow 0$ then $g(x) \rightarrow \mathbb{R}$. Therefore, $\big|(0,1]\big| = \big| \mathbb{R} \big|$.

* 6
** Problem Statement
Show that the intersection of a convex set is convex.

** Solution
Let $A$ and $B$ be two convex sets, and let $C = A \cup B$. Now let $p,q \in C$.

- If $p,q \in C$ then $p,q \in A$ and $A$ is convex
- If $p,q \in C$ then $p,q \in B$ and $B$ is convex
- Therefore $C$ must be complex

* 7
** Problem Statement
If $S$ and $T$ are convex sets both in $\mathbb{R}^n$, show that the set sum is convex.

#+attr_latex: :width 0.45\textwidth
[[./img/set-sum.png]]

** Solution
The set sum is defined as

$$
S+T = \{x: x = s + t, s\in S, t \in T\}
$$

Let $S$ and $T$ be convex sets and $S+T \in C$, let $s_1, s_2 \in S$ and $t_1, t_2 \in T$, and let $s = s_1 + t_1$ and $t = s_2 + t_2$, then

\begin{equation*}
\lambda s + (1 - \lambda)t \\
\lambda s_1 + \lambda t_1 + s_2(1-\lambda) + t_2(1-\lambda) \\
\lambda s_1 + (1-\lambda)t_1 + \lambda s_2 + (1-\lambda) t_2 \in C \\
\end{equation*}

Therefore, the set sum is convex.

* 8
:PROPERTIES:
:CUSTOM_ID: sec:1.8
:END:
** Problem Statement
Show that the polytope in $n$ dimensions is defined by

\begin{equation*}
P_n = \{ x \in \mathbb{R}^n : x_i \ge 0, \sum_{i=1}^n x_i = 1 \}
\end{equation*}

** Solution
Let is take the case of $n=1$ to start. Let $p = x1$ and $q = y_1$ then
using the definition used before we get

$$
\lambda p + (1 - \lambda)q
$$

Which must be convex because it is a single point. Now let $n=3$

\begin{equation*}
\begin{array}{c}
\lambda p + (1 - \lambda)q \\
\lambda (x_1, x_2, x_3) + (1 - \lambda)(y_1, y_2, y_2) = (z_1, z_2, z_3)\\
\end{array}
\end{equation*}

Because $z$ must add up to 1, the set must be convex.

* 9
** Problem Statement
For the polytope $P_n$ of the previous problem, let $(a_1, a_2, \cdots, a_n) \in P_n$. Show by induction that

$$
n^2 \le \sum_{i=1}^n \frac{1}{a_i}
$$

** Solution
Begin with the base case, $n=1$.

\begin{equation*}
\begin{array}{c}
1^2 \le \sum_{i=1}^1 \frac{1}{1} \\
1 \le 1
\end{array}
\end{equation*}

which is true. Now let

$$
n^2 \le \sum_{i=1}^n \frac{1}{a_i}
$$

be true. We now need to show that the following is true

$$
(n+1)^2 \le \sum_{i=1}^{n+1} \frac{1}{a_i}
$$

Begin by defining an element from $P_N$: $p = (a_1, a_2, \cdots, a_n)$. To make $p$ an element in the $P_{n+1}$ space let $p
= (a_1, a_2, \cdots, a_n, 0)$. Let's define another point $q = (0, 0, \cdots, 0, 1)$. Now let's define the line between the points
$p$ and $q$

\begin{equation*}
\begin{array}{c}
\lambda p + (1 - \lambda)q \\
\lambda (a_1, a_2, \cdots, a_n, 0) + (1 - \lambda)(0, 0, \cdots, 0, 1) = (b_1, b_2, \cdots, b_{n+1}) \\
\end{array}
\end{equation*}

Going back to the $(n+1)^2 \le \sum_{i=1}^{n+1} \frac{1}{a_i}$, let's plug this in for $b$ for $a$: $(n+1)^2 = \sum_{i=1}^{n+1}
\frac{1}{b_i}$. Note that the $(1-\lambda)$ is non-zero at $n+1$, so we can rewrite this as $(n+1)^2 = \frac{1}{1-\lambda} + \sum_{i=1}^{n+1}
\frac{1}{\lambda a_i}$. Now to remove the $\lambda$:

\begin{equation*}
\frac{1}{1-\lambda} + \sum_{i=1}^{n+1} \frac{1}{\lambda a_i} \le \sum_{i=1}^{n+1} \frac{1}{a_i} \\
\end{equation*}

Therefore, $(n+1)^2 \le \sum_{i=1}^{n+1} \frac{1}{a_i}$.

* 10
** Problem Statement
Show that $(AB)^T = B^T A^T$ is true.

** Solution
Let $A$ be a $m \times n$ matrix and $B$ be a $n \times p$ matrix. And let $A = (a_{ij})$ and $A^T = (a_{ji})$, the same can be
said for $B$. If we look at the multiplication of $(AB)^T$

$$
(AB)^T = \sum_{k=1}^n (a_{ik} b_{ki})^T
$$

Which denotes the row/column multiplication/addition of matrix multiplication for transposed matrices. Now if we
transpose the summed values

$$
(AB)^T = \sum_{k=1}^n (a_{ik} b_{ki})^T = \sum_{k=1}^n (a_{kj} b_{ki})
$$

Reversing the multiplication order we get

$$
(AB)^T = \sum_{k=1}^n (b_{ki} a_{kj})^T = B^T A^T
$$

* 11
** Problem Statement
Show that the following are true

** Solution

*** $A_{i:} = \sum_j a_{ij}e_{j}$
Begin with definition of unit vectors

\begin{equation*}
\begin{array}{ccc}
e_1 =
\begin{bmatrix}
1 \\ 0 \\ 0 \\ \vdots \\ 0
\end{bmatrix}
e_2 =
\begin{bmatrix}
0 \\ 1 \\ 0 \\ \vdots \\ 0
\end{bmatrix}
e_n =
\begin{bmatrix}
0 \\ 0 \\ 0 \\ \vdots \\ n
\end{bmatrix}
\end{array}
\end{equation*}

Now outline the form of $A_{i:} = [a_{i1},a_{i2},a_{i3},\cdots,a_{in}]$ which denotes the all the elements of row $i$. To
show that is equivalent to the sum, begin by expanding the sum. Let $k$ be the column of interest.

\begin{equation*}
\sum_j a_{ij}e_j = a_{i1}e_1 + a_{i2}e_2 + \cdots + a_{ik}e_{k} + a_{in}e_n
\end{equation*}

Referring back to the definition of $e$, we see that only $e_k$ is nonzero therefore the only value returned is
$a_{ik}$. Extrapolating this for all columns $n$ in the matrix we get the vector $[a_{i1},a_{i2},a_{i3},\cdots,a_{in}]$.

*** $A_{:j} = \sum_i a_{ij}e_{i}$
This is very similarly to the previous problem; however, now we are summing over the columns. $A_{:j} = [a_{1j},a_{2j}
\cdots,a_{mj}]^T$. Now taking the sum version, we find

\begin{equation*}
\sum_i a_{ij}e_i = a_{1j}e_1 + a_{2j}e_2 + \cdots + a_{kj}e_{k} + a_{nj}e_m
\end{equation*}

Where the only nonzero value in $e$ is $e_k$, therefore we are returned $a{kj}$ when $i=k$. Doing this for all $m$
elements returns the vector $[a_{1j},a_{2j},\cdots,a_{mj}]^T$

*** $A_{i:}^T = \sum_j a_{ij}e_{j}^T$
This is nearly the same as $A_{i:} = \sum_j a_{ij}e_{j}$, but now because $A$ is transposed, the unit vectors must also be
transposed to keep the dimensions connect (column vector to row). Therefore, in a similar vein we can state $(A_{i:}^T)
= (a_{:i}) = [a_{1i},a_{2i},\cdots,a_{ni}]^T$. Taking the summed version we find

\begin{equation*}
\sum_j a_{ij}e_j^T = a_{1i}e_1 + a_{2i}e_2 + \cdots + a_{ki}e_{k} + a_{ni}e_n
\end{equation*}

Again, because $k$ is the index of interest the only value that is returned is $a_{ki}$. Extrapolating out, as we have
done before, we find that the vector that is returned is the column vector of $[a_{1i},a_{2i},\cdots,a_{ni}]^T$.

* 12
** Problem Statement
Show that $(A^{-1})^T = (A^T)^{-1}$.

** Solution
Let $A^{-1} = B$. Then we can write

$$
B^T = (A^T)^{-1}
$$

Inverting both sides and stating the fact that $(A^{-1})^{-1} = A$ we get

$$
A^T = (B^T)^{-1}
$$

Substituting the result from above back into the original equation we get

$$
((B^T)^{-1})^{-1} = B^T
$$

Using the definition that the inverse of an inverse is the original matrix for an inverterable matrix we get

$$
B^T = B^T
$$

Therefore, $(A^{-1})^T = (A^T)^{-1}$.

* 13
** Problem Statement
Show that $\text{tr}(AB) = \text{tr}(BA)$

** Solution
Define what the trace of a matrix is

#+begin_quote
The trace of a matrix $\text{tr}(A) = \sum_{i=1}^{n} a_{ii}$. In other words, the trace is the sum of the elements along
the main of the diagonal
#+end_quote

The trace can be written as

$$
\text{tr}(AB) = (AB)_{ii} = \sum_{k=1}^m (AB)_{ii} = \sum_{i=1}^m \sum_{k=1}^n A_{ik} B_{ki}
$$

Reversing the summations we get

$$
\sum_{k=1}^n \sum_{i=1}^m B_{ki} A_{ik} = \sum_{k=1}^n (BA)_{kk} = \text{tr}(BA)
$$

* 14
** Problem Statement
Define the offset trace as a generalization of the usual trace

$$
\text{tr}(C,l) = \sum_{i} C_{i,i+l}
$$

where the usual trace is obtained when $l = 0$, and for $l > 0$, the sum is taken on the $l\text{th}$ superdiagonal. Show that
for $l \ne 0$

$$
\text{tr}(AB, l) = \text{tr}(B^T A^T, l)
$$

** Solution
To begin we state the fact that was proven before.

$$
(AB)^T = B^T A^T
$$

Now we need to show that $(A)_{i,i+1} = ((A)_{i+1, i})^T$. The obvious case is when $j=0$, when $l>0$. Let $j = i+l$, we
know that

$$
(a_{i,j}) = (a_{j,i})^T
$$

substituting $j=i+1$ is then obvious. Putting these facts together, let $C=AB$

$$
\text{tr}(C,l) = \sum_{i} C^T_{i+l,i} = \sum_{i} (B^T A^T)_{i+l,i}
$$

* 15

** Problem Statement
Let two complex numbers be defined as $z_1 = a + jb$ and $z_2 = c + jd$. Let $z_3 = z_1 z_2 = e + jf$. Show

1. The product can be written as

\begin{equation*}
\begin{bmatrix} e \\ f \end{bmatrix} =
\begin{bmatrix} c & -d \\ d & c \end{bmatrix}
\begin{bmatrix} a \\ b \end{bmatrix}
\end{equation*}

2. The complex product can also be written as

\begin{equation*}
\begin{array}{cc}
e = (a-b)d + a(c-d) & f = (a-b)d + b(c+d)
\end{array}
\end{equation*}

3. Show that this modified scheme can be expressed in matrix notation as

\begin{equation*}
\begin{bmatrix} e \\ f \end{bmatrix} =
\begin{bmatrix} 1 & 0 & 1 \\ 0 & 1 & 1 \end{bmatrix}
\begin{bmatrix}
(c-d) & 0 & 0 \\
0 & (c+d) & 0 \\
0 & 0 & d
\end{bmatrix}
\begin{bmatrix}
1 & 0 \\
0 & 1 \\
1 & -1
\end{bmatrix}
\begin{bmatrix} a \\ b \end{bmatrix}
\end{equation*}

** Solution

*** 1.4-1.1
Complex matrix multiplication can be written as

$$
z_1 z_2 = (a+jb)(c+jd)
$$

Expanding and combining real and imaginary terms

\begin{equation*}
\begin{array}{c}
z_1 z_2 = ac + ajd + cjb + bdj^2 \\
(ac - bd) + (ajd + cjb)
\end{array}
\end{equation*}

Now lets expand the matrix form shown in the problem statement

\begin{equation*}
\begin{bmatrix} e \\ f \end{bmatrix} =
\begin{bmatrix} c & -d \\ d & c \end{bmatrix}
\begin{bmatrix} a \\ b \end{bmatrix} =
\begin{bmatrix}
ca - bd \\ da + cb
\end{bmatrix}
\end{equation*}

Note that the grouped pairs match for real and imaginary parts.

*** 1.4-1.2
This can be found by simply expanding and simplifying. Lets begin with $e$

\begin{equation*}
\begin{array}{l}
e = (a-b)d + a(c-d) \\
e = ad - bd + ac - ad \\
e = ac - bd
\end{array}
\end{equation*}

Which matches the two solutions found before. Similarly for $f$

\begin{equation*}
\begin{array}{l}
f = (a-b)d + b(c+d) \\
f = ad - bd + bc + bd \\
f = ad + bc
\end{array}
\end{equation*}

Which, again, matches what was found before.

*** 1.4-1.3
Once again, we can show that they are equivalent by expansion and simplification. We will work from left to right
performing matrix multiplication

\begin{equation*}
\begin{array}{c}
\begin{bmatrix} e \\ f \end{bmatrix} =
\begin{bmatrix} 1 & 0 & 1 \\ 0 & 1 & 1 \end{bmatrix}
\begin{bmatrix}
(c-d) & 0 & 0 \\
0 & (c+d) & 0 \\
0 & 0 & d
\end{bmatrix}
\begin{bmatrix}
1 & 0 \\
0 & 1 \\
1 & -1
\end{bmatrix}
\begin{bmatrix} a \\ b \end{bmatrix} \\
\begin{bmatrix} e \\ f \end{bmatrix} =
\begin{bmatrix}
(c-d) & 0 & d \\
0 & (c+d) & d \\
\end{bmatrix}
\begin{bmatrix}
1 & 0 \\
0 & 1 \\
1 & -1
\end{bmatrix}
\begin{bmatrix} a \\ b \end{bmatrix} \\
\begin{bmatrix} e \\ f \end{bmatrix} =
\begin{bmatrix}
(c-d) & -d \\
d & c \\
\end{bmatrix}
\begin{bmatrix} a \\ b \end{bmatrix} =
\begin{bmatrix}
ca - bd \\ da + cb
\end{bmatrix}
\end{array}
\end{equation*}

Which is equivalent to what was found in the previous problems.

* 16

** Problems Statement
Show that

$$
k_j = \frac{1}{p^j j!}(-1)^j \frac{d^j}{d(z^{-1})^j} (1-pz^-1)^r H(z) \Big|_{z=p}
$$

for the partial fraction expansion of a Z-transform with repeated roots is correct.

** Solution
